Jeszcze trochę dłubania w pochodnych Brzozowskiego.

code/Brzozowski.v
@@ -1,8 +1,14 @@
 (** Zainspirowane przez http://www.weaselhat.com/2020/05/07/smart-constructors-are-smarter-than-you-think/
-    Definicje wzięte z https://en.wikipedia.org/wiki/Brzozowski_derivative *)
+    Definicje wzięte z https://en.wikipedia.org/wiki/Brzozowski_derivative
+
+    Zobacz też: https://semantic-domain.blogspot.com/2013/11/antimirov-derivatives-for-regular.html *)
 
 Set Implicit Arguments.
 Set Maximal Implicit Insertion.
+
+Require Import Bool.
+Require Import List.
+Import ListNotations.
 
 Inductive Regex (A : Type) : Type :=
     | Empty : Regex A
@@ -32,7 +38,7 @@ Fixpoint aux
   : Regex A :=
 match r with
     | Empty   => Empty
-    | Epsilon => Epsilon
+    | Epsilon => Empty
     | Char x  => if dec a x then Epsilon else Empty
     | Seq r1 r2 =>
         Or (Seq (aux dec a r1) r2)
@@ -42,9 +48,6 @@ match r with
     | Or r1 r2 => Or (aux dec a r1) (aux dec a r2)
     | Star r' => Seq (aux dec a r') (Star r')
 end.
-
-Require Import List.
-Import ListNotations.
 
 Fixpoint brzozowski
   {A : Type} (dec : A -> A -> bool)
@@ -59,12 +62,6 @@ Definition matches
   {A : Type} (dec : A -> A -> bool)
   (l : list A) (r : Regex A) : bool :=
     containsEpsilon (brzozowski dec (rev l) r).
-
-Fixpoint repeat {A : Type} (n : nat) (l : list A) : list A :=
-match n with
-    | 0 => []
-    | S n' => l ++ repeat n' l
-end.
 
 Inductive Matches {A : Type} : list A -> Regex A -> Prop :=
     | MEpsilon : Matches [] Epsilon
@@ -89,8 +86,6 @@ Ltac inv H := inversion H; subst; clear H; auto.
 
 Hint Constructors Matches : core.
 
-Require Import Bool.
-
 Lemma containsEpsilon_Matches_nil :
   forall
     {A : Type} (r : Regex A),
@@ -99,39 +94,16 @@ Lemma containsEpsilon_Matches_nil :
       Matches [] r.
 Proof.
   split.
-    induction r; cbn.
-      inversion 1.
-      constructor.
-      inversion 1.
-      intro. destruct (containsEpsilon r1), (containsEpsilon r2); inv H.
-        change [] with (@nil A ++ []). constructor.
-          apply IHr1. reflexivity.
-          apply IHr2. reflexivity.
-      intros. destruct (containsEpsilon r1); cbn in *; eauto.
-      change (@nil A) with (@repeat A 0 []). constructor.
-    induction r; cbn; intros.
-      inv H.
-      reflexivity.
-      inv H.
-      inv H. rewrite IHr1, IHr2.
-        reflexivity.
-        destruct l1, l2; inv H0.
-        destruct l1, l2; inv H0.
-      inv H.
-        rewrite IHr1; auto.
-        rewrite IHr2.
+    induction r; cbn; intros; inv H.
+      destruct (containsEpsilon r1), (containsEpsilon r2); inv H1.
+        change [] with (@nil A ++ []). auto.
+      destruct (containsEpsilon r1); cbn in *; auto.
+    induction r; cbn; intros; inv H.
+      destruct l1, l2; inv H0. rewrite IHr1, IHr2; auto.
+      rewrite IHr1; auto.
+      rewrite IHr2.
           apply orb_true_r.
           assumption.
-      reflexivity.
-Qed.
-
-Lemma repeat_nil :
-  forall {A : Type} (n : nat),
-    @repeat A n [] = [].
-Proof.
-  induction n as [| n']; cbn.
-    reflexivity.
-    rewrite IHn'. reflexivity.
 Qed.
 
 Lemma Matches_aux :
@@ -142,24 +114,18 @@ Lemma Matches_aux :
         forall (h : A) (t : list A),
           l = h :: t -> Matches t (aux dec h r).
 Proof.
-  induction 1; cbn; intros.
-    inv H.
-    inv H. cbn. admit.
+  induction 1; cbn; intros h t Heq.
+    inv Heq.
+    inv Heq. cbn. admit.
     destruct l1 as [| h1 t1]; cbn in *.
       subst. specialize (IHMatches2 _ _ eq_refl).
         rewrite <- containsEpsilon_Matches_nil in H. rewrite H. auto.
-        inv H1.
+        inv Heq.
     auto.
     auto.
-    inv H.
-    {
-      destruct l1 as [| h1 t1]; inv H1.
-      specialize (IHMatches2 _ _ H2).
-      inversion IHMatches2; subst.
-      constructor.
-        assumption.
-        assumption.
-    }
+    inv Heq.
+    destruct l1 as [| h1 t1]; inv Heq.
+      specialize (IHMatches2 _ _ H1). inv IHMatches2.
 Admitted.
 
 Lemma Matches_aux' :
@@ -171,7 +137,7 @@ Proof.
   intros until r. revert h t.
   induction r; cbn; intros.
     inv H.
-    admit.
+    inv H.
     destruct (dec h a) eqn: Hdec.
       inv H. admit.
       inv H.
@@ -220,25 +186,298 @@ Proof.
       eapply Matches_aux'. eassumption.
 Qed.
 
+Lemma Matches_brzozowski'' :
+  forall
+    {A : Type} (dec : A -> A -> bool)
+    (l1 l2 : list A) (r : Regex A),
+      Matches l2 (brzozowski dec l1 r)
+        <->
+      Matches (rev l1 ++ l2) r.
+Proof.
+  induction l1 as [| h1 t1]; cbn; intros.
+    reflexivity.
+    rewrite <- app_assoc, <- IHt1. cbn. Check Matches_aux.
+Restart.
+  split; revert l2 r.
+    induction l1 as [| h1 t1]; cbn; intros.
+      assumption.
+      rewrite <- app_assoc. apply IHt1. cbn.
+        eapply Matches_aux'. eassumption.
+    induction l1 as [| h1 t1]; cbn; intros.
+      assumption.
+      eapply Matches_aux.
+        2: reflexivity.
+        apply IHt1. rewrite <- app_assoc in H. cbn in H. assumption.
+Qed.
+
 Lemma Matches_matches :
   forall
     {A : Type} (dec : A -> A -> bool)
     (l : list A) (r : Regex A),
       Matches l r <-> matches dec l r = true.
 Proof.
-  split.
-    {
-      intros. unfold matches.
-      rewrite containsEpsilon_Matches_nil.
-      eapply Matches_brzozowski.
-        exact H.
-        rewrite rev_involutive, app_nil_r. reflexivity.
-    }
-    {
-      unfold matches. intros.
-      rewrite containsEpsilon_Matches_nil in H.
-      apply Matches_brzozowski' in H.
-      rewrite rev_involutive, app_nil_r in H.
-      assumption.
-    }
+  intros. unfold matches.
+  rewrite containsEpsilon_Matches_nil.
+  rewrite Matches_brzozowski''.
+  rewrite rev_involutive, app_nil_r.
+  reflexivity.
 Qed.
+
+Require Import Equality.
+
+Scheme Matches_ind' := Induction for Matches Sort Prop.
+
+(* Not true. *)
+Lemma isProp_Matches :
+  forall
+    {A : Type} (l : list A) (r : Regex A)
+    (m1 m2 : Matches l r),
+      m1 ~= m2.
+Proof.
+  induction m1 using @Matches_ind'; intros.
+    dependent destruction m2. reflexivity.
+    dependent destruction m2. reflexivity.
+    dependent destruction m2. rewrite <- x.
+Abort.
+
+Fixpoint repeat {A : Type} (n : nat) (x : A) : list A :=
+match n with
+    | 0    => []
+    | S n' => x :: repeat n' x
+end.
+
+(* 0.001 sec *)
+(* Time Compute matches eqb (repeat 10 true) (Star (Char true)). *)
+
+(* 1.9 sec *)
+(* Time Compute matches eqb (repeat 20 true) (Star (Char true)). *)
+
+(* timeout *)
+(* Time Compute matches eqb (repeat 30 true) (Star (Char true)). *)
+
+(* * Same thing, but using smart constructors. *)
+
+Definition empty {A : Type} : Regex A := Empty.
+
+Definition epsilon {A : Type} : Regex A := Epsilon.
+
+Definition char {A : Type} (x : A) : Regex A := Char x.
+
+Definition seq {A : Type} (r1 r2 : Regex A) : Regex A :=
+match r1, r2 with
+    | Empty  , _       => Empty
+    | _      , Empty   => Empty
+    | Epsilon, _       => r2
+    | _      , Epsilon => r1
+    | _      , _       => Seq r1 r2
+end.
+
+Print Regex.
+
+Definition or {A : Type} (r1 r2 : Regex A) : Regex A :=
+match r1, r2 with
+    | Empty, _ => r2
+    | _, Empty => r1
+    | Epsilon, _ => if containsEpsilon r2 then r2 else Or r1 r2
+    | _, Epsilon => if containsEpsilon r1 then r1 else Or r1 r2
+    | _, _ => Or r1 r2
+end.
+
+Definition star {A : Type} (r : Regex A) : Regex A :=
+match r with
+    | Empty => Epsilon
+    | Epsilon => Epsilon
+    | Star r' => Star r'
+    | _ => Star r
+end.
+
+Fixpoint aux'
+  {A : Type} (dec : A -> A -> bool)
+  (a : A) (r : Regex A)
+  : Regex A :=
+match r with
+    | Empty   => empty
+    | Epsilon => empty
+    | Char x  => if dec a x then epsilon else empty
+    | Seq r1 r2 =>
+        or (seq (aux' dec a r1) r2)
+           (if containsEpsilon r1
+            then aux' dec a r2
+            else empty)
+    | Or r1 r2 => or (aux' dec a r1) (aux' dec a r2)
+    | Star r' => seq (aux' dec a r') (star r')
+end.
+
+Fixpoint brzozowski'
+  {A : Type} (dec : A -> A -> bool)
+  (l : list A) (r : Regex A)
+  : Regex A :=
+match l with
+    | [] => r
+    | h :: t => aux' dec h (brzozowski' dec t r)
+end.
+
+Definition matches'
+  {A : Type} (dec : A -> A -> bool)
+  (l : list A) (r : Regex A) : bool :=
+    containsEpsilon (brzozowski' dec (rev l) r).
+
+
+(* Time Compute matches' eqb (repeat 10 true) (Star (Char true)). *)
+(* ===> Finished transaction in 0. secs (0.u,0.s) (successful) *)
+
+(* Time Compute matches' eqb (repeat 20 true) (Star (Char true)). *)
+(* ===> Finished transaction in 0. secs (0.u,0.s) (successful) *)
+
+(* Time Compute matches' eqb (repeat 40 true) (Star (Char true)). *)
+(* ===> Finished transaction in 0.001 secs (0.001u,0.s) (successful) *)
+
+(* Time Compute matches' eqb (repeat 80 true) (Star (Char true)). *)
+(* ===> Finished transaction in 0.001 secs (0.u,0.001s) (successful) *)
+
+(* Time Compute matches' eqb (repeat 160 true) (Star (Char true)). *)
+(* ===> Finished transaction in 0.003 secs (0.002u,0.001s) (successful) *)
+
+(* Time Compute matches' eqb (repeat 320 true) (Star (Char true)). *)
+(* ===> Finished transaction in 0.013 secs (0.007u,0.001s) (successful) *)
+
+(* Time Compute matches' eqb (repeat 640 true) (Star (Char true)). *)
+(* ===> Finished transaction in 0.046 secs (0.024u,0.002s) (successful) *)
+
+(* Time Compute matches' eqb (repeat 1280 true) (Star (Char true)). *)
+(* ===> Finished transaction in 0.125 secs (0.063u,0.002s) (successful) *)
+
+(* Time Compute matches' eqb (repeat 2560 true) (Star (Char true)). *)
+(* ===> Finished transaction in 0.305 secs (0.191u,0.001s) (successful) *)
+
+(* Time Compute matches' eqb (repeat 5120 true) (Star (Char true)). *)
+(* ===> Finished transaction in 0.984 secs (0.694u,0.004s) (successful) *)
+
+Require Import FunInd.
+
+Function optimize {A : Type} (r : Regex A) : Regex A :=
+match r with
+    | Empty => Empty
+    | Epsilon => Epsilon
+    | Char x => Char x
+    | Seq r1 r2 =>
+        match optimize r1, optimize r2 with
+            | Empty, _ => Empty
+            | _, Empty => Empty
+            | Epsilon, r2' => r2'
+            | r1', Epsilon => r1'
+            | r1', r2' => Seq r1' r2'
+        end
+    | Or r1 r2 =>
+        match optimize r1, optimize r2 with
+            | Empty, r2' => r2'
+            | r1', Empty => r1'
+            | Epsilon, r2' => if containsEpsilon r2' then r2' else Or Epsilon r2'
+            | r1', Epsilon => if containsEpsilon r1' then r1' else Or r1' Epsilon
+            | r1', r2' => Or r1' r2'
+        end
+    | Star r' =>
+        match optimize r' with
+            | Empty => Epsilon
+            | Epsilon => Epsilon
+            | Star r'' => Star r''
+            | r'' => Star r''
+        end
+end.
+
+Definition matches''
+  {A : Type} (dec : A -> A -> bool)
+  (l : list A) (r : Regex A) : bool :=
+    containsEpsilon (optimize (brzozowski' dec (rev l) r)).
+
+(* Time Compute matches'' eqb (repeat 5120 true) (Star (Char true)). *)
+(* ===> Finished transaction in 0.733 secs (0.594u,0.001s) (successful) *)
+
+(* Time Compute matches'' eqb (repeat 10240 true) (Star (Char true)). *)
+(* ===> Finished transaction in 4.028 secs (2.599u,0.051s) (successful) *)
+
+Lemma optimize_Empty :
+  forall {A : Type} (r : Regex A),
+    optimize r = Empty -> forall l : list A, ~ Matches l r.
+Proof.
+  intros A r. unfold not.
+  functional induction optimize r; intros H l HM;
+  inv H; inv HM; eauto.
+    rewrite H1 in y. contradiction.
+    rewrite H1 in y. contradiction.
+Qed.
+
+Lemma optimize_Epsilon :
+  forall {A : Type} (r : Regex A),
+    optimize r = Epsilon -> forall l : list A, Matches l r -> l = [].
+Proof.
+  intros A r.
+  functional induction optimize r; intros H l HM;
+  inv H; inv HM; eauto.
+    rewrite (IHr0 e0 _ H3), (IHr1 H1 _ H4). reflexivity.
+    rewrite (IHr0 H1 _ H3), (IHr1 e1 _ H4). reflexivity.
+    contradict H2. apply optimize_Empty. assumption.
+    contradict H2. apply optimize_Empty. assumption.
+    contradict H0. apply optimize_Empty. assumption.
+    rewrite (IHr0 e0 _ H0). cbn. functional inversion e0; subst.
+      destruct l2.
+        reflexivity.
+        inv H2. destruct l0; inv H.
+Admitted.
+
+Lemma Matches_optimize :
+  forall {A : Type} (l : list A) (r : Regex A),
+    Matches l r <-> Matches l (optimize r).
+Proof.
+  intros. revert l.
+  functional induction optimize r; intros.
+    1-3: firstorder.
+    split; intro H; inv H. contradict H3. apply optimize_Empty. assumption.
+    split; intro H; inv H. contradict H4. apply optimize_Empty. assumption.
+
+    rewrite <- IHr1. split; intro H.
+      inv H. apply optimize_Epsilon in H3; subst; cbn; assumption.
+      change l with ([] ++ l). constructor.
+        rewrite IHr0, e0. constructor.
+        assumption.
+    rewrite <- IHr0. split; intro H.
+      inv H. apply optimize_Epsilon in H4; subst; cbn.
+        rewrite app_nil_r. assumption.
+        assumption.
+      rewrite <- (@app_nil_r A l). constructor.
+        assumption.
+        rewrite IHr1, e1. constructor.
+    split; intro H; inv H; constructor; rewrite <- ?IHr0, <- ?IHr1 in *; assumption.
+    rewrite <- IHr1. split; intro H; inv H. apply optimize_Empty in H2; firstorder.
+    rewrite <- IHr0. split; intro H; inv H. apply optimize_Empty in H2; firstorder.
+    rewrite <- IHr1. split; intro H; inv H. apply optimize_Epsilon in H2; subst.
+      rewrite IHr1, <- containsEpsilon_Matches_nil. assumption.
+      assumption.
+    split; intro H; inv H.
+      constructor. apply optimize_Epsilon in H2; subst; auto.
+      constructor 5. rewrite <- IHr1. auto.
+      constructor. rewrite IHr0, e0. assumption.
+      constructor 5. rewrite IHr1. assumption.
+    rewrite <- IHr0. split; intro H.
+      inv H. apply optimize_Epsilon in H2; subst; auto.
+        rewrite containsEpsilon_Matches_nil, <- IHr0 in e2. assumption.
+      constructor. assumption.
+    split; intro H; inv H.
+      constructor. rewrite <- IHr0. assumption.
+      constructor 5. apply optimize_Epsilon in H2; subst; auto.
+      constructor. rewrite IHr0. assumption.
+      constructor 5. rewrite IHr1, e1. assumption.
+    split; intro H; inv H.
+      constructor. rewrite <- IHr0. assumption.
+      constructor 5. rewrite <- IHr1. assumption.
+      constructor. rewrite IHr0. assumption.
+      constructor 5. rewrite IHr1. assumption.
+    split; intro H; inv H. rewrite IHr0, e0 in H1. inv H1.
+    {
+      split; intro H; inv H.
+      apply optimize_Epsilon in H1; subst; cbn; auto.
+      apply optimize_Epsilon in H3; subst; cbn.
+        constructor.
+        rewrite e0. reflexivity.
+    }
+Abort.
